test/artifact/security/Crypto.AEAD.Encoding.fst
@@ -60,9 +60,9 @@ let rec encode_bytes txt =
     Seq.createEmpty
   else 
     let l0 = min l 16 in
-    let txt0, txt = SeqProperties.split txt l0 in
+    let txt0, txt = Seq.split txt l0 in
     let w = pad_0 txt0 (16 - l0) in 
-    SeqProperties.cons w (encode_bytes txt)
+    Seq.cons w (encode_bytes txt)
 
 #reset-options "--lax"
 let rec lemma_encode_length txt: Lemma
@@ -73,7 +73,7 @@ let rec lemma_encode_length txt: Lemma
   if l = 0 then ()
   else if l < 16 then assert(Seq.length(encode_bytes txt) = 1)
   else (
-    let txt0, txt' = SeqProperties.split txt 16 in
+    let txt0, txt' = Seq.split txt 16 in
     lemma_encode_length txt';
     assume false;
     assert(Seq.length(encode_bytes txt) = 1 + Seq.length(encode_bytes txt')))
@@ -94,7 +94,7 @@ val lemma_pad_0_injective: b0:Seq.seq UInt8.t -> b1:Seq.seq UInt8.t -> l:nat -> 
   (requires (pad_0 b0 l == pad_0 b1 l))
   (ensures  (b0 == b1))
 let lemma_pad_0_injective b0 b1 l =
-  SeqProperties.lemma_append_inj b0 (Seq.create l 0uy) b1 (Seq.create l 0uy);
+  Seq.lemma_append_inj b0 (Seq.create l 0uy) b1 (Seq.create l 0uy);
   Seq.lemma_eq_intro b0 b1
 
 #reset-options "--initial_fuel 1 --max_fuel 1 --initial_ifuel 0 --max_ifuel 0"
@@ -209,8 +209,8 @@ private let encode_lengths (i:id) (aadlen:aadlen_32) (txtlen:txtlen_32) : lbytes
   | GHASH    -> encode_lengths_ghash aadlen txtlen
 
 let encode_both (i:id) (aadlen:aadlen_32) (aad:lbytes (v aadlen)) (txtlen:txtlen_32) (cipher:lbytes (v txtlen)) :
-  e:MAC.text {Seq.length e > 0 /\ SeqProperties.head e = encode_lengths i aadlen txtlen} = 
-  SeqProperties.cons (encode_lengths i aadlen txtlen)
+  e:MAC.text {Seq.length e > 0 /\ Seq.head e = encode_lengths i aadlen txtlen} = 
+  Seq.cons (encode_lengths i aadlen txtlen)
     (Seq.append 
       (encode_bytes cipher) 
       (encode_bytes aad))
@@ -221,7 +221,6 @@ let lemma_encode_both_inj i (al0:aadlen_32) (pl0:txtlen_32) (al1:aadlen_32) (pl1
   (ensures al0 = al1 /\ pl0 = pl1 /\ a0 = a1 /\ p0 = p1) = 
 
   let open FStar.Seq in 
-  let open FStar.SeqProperties in
   let w0 = encode_lengths i al0 pl0 in 
   let w1 = encode_lengths i al1 pl1 in
   //assert(encode w0 = encode w1);
